rocq/common/relations.v
@@ -30,7 +30,7 @@ Proof.
 Qed.
 
 
-(* Iterate a step relation n-times *)
+(* Iterate a step relation *exactly* n-times *)
 Inductive step_n {A} (step : A -> A -> Prop) : nat -> A -> A -> Prop := 
   | s_done e : 
     step_n step 0 e e
@@ -39,7 +39,36 @@ Inductive step_n {A} (step : A -> A -> Prop) : nat -> A -> A -> Prop :=
     step_n step k e2 e3 -> 
     step_n step (S k) e1 e3.
 
-(* 
-Lemma step_n_app {A} (step : A -> A -> Prop) k1 k2 e1 e2 e3 :
-  step_n step k1 e1 e2 -> step_n step k2 e2 e3 -> step_n step (k1 + k2) e1 e3.
-*)
+Arguments s_done {_}{_}{_}.
+Arguments s_next {_}{_}{_}{_}{_}.
+
+
+Lemma s_done' {A} (step : A -> A -> Prop) e1 e2 : 
+  e1 = e2 -> step_n step 0 e1 e2.
+Proof.  intro. subst. eapply s_done. Qed.
+
+Lemma s_one' {A} (step : A -> A -> Prop) e1 e2 :
+  step e1 e2 -> step_n step 1 e1 e2.
+Proof. intros. eapply s_next; eauto. eapply s_done. Qed.
+
+Lemma s_app {A} (step : A -> A -> Prop) k1 k2 e1 e2 e3 :
+  step_n step k1 e1 e2 -> step_n step k2 e2 e3 -> 
+  step_n step (k1 + k2) e1 e3.
+Proof.
+  intros h1 h2.
+  induction h1; cbn; eauto.
+  eapply s_next; eauto.
+Qed.
+
+Lemma step_n_multi {A} (step : A -> A -> Prop) n e1 e2 :
+  step_n step n e1 e2 -> multi step e1 e2.
+Proof.
+  induction 1; econstructor; eauto.
+Qed.
+
+Lemma multi_step_n {A} (step : A -> A -> Prop) e1 e2 :
+  multi step e1 e2 -> exists n, step_n step n e1 e2.
+Proof.
+  induction 1. eexists; econstructor; eauto.
+  destruct IHmulti. eexists; econstructor; eauto.
+Qed.
