rocq/untyped/ctx.v
@@ -1,0 +1,225 @@
+From Stdlib Require Import Psatz.
+From Stdlib Require Import Arith.
+
+Require Export common.core.
+Require Export untyped.stack.
+
+Import Lists.List.ListNotations.
+Import SyntaxNotations.
+Import stack.Notations.
+
+Open Scope list_scope.
+Open Scope rec_scope.
+
+
+(* --------------------------------------------------------- *)
+
+Definition scoped_relation (T : nat -> Type) := forall n, T n -> T n -> Prop.
+
+Class Reflexive {T : nat -> Type} (R : scoped_relation T) : Prop := 
+  { scoped_refl : forall n x, R n x x }.
+
+Class Transitive {T : nat -> Type} (R : scoped_relation T) : Prop := 
+  { scoped_trans : forall n (t1 t2 t3 : T n), R _ t1 t2 -> R _ t2 t3 -> R _ t1 t3 }.
+
+Class PreOrder {T : nat -> Type} (R : scoped_relation T) := 
+  { po_scoped_refl  : Reflexive R ;
+    po_scoped_trans : Transitive R
+  }.
+
+Definition Adequate (RE : scoped_relation Tm) := 
+  forall (e e' : Tm 0), RE _ e e' -> Small.halts (nil, e) -> Small.halts (nil, e').
+
+Existing Class Adequate.
+
+Class Compatible (RE : scoped_relation Tm) (RV : scoped_relation Val) := 
+  { val_var n x :
+      RV n (var x) (var x) ;
+
+    val_unit n : 
+      RV n unit unit ;
+
+    val_zero n : 
+      RV n zero zero ;
+
+    val_succ n x y :
+      RV n x y ->
+      RV n (succ x) (succ y) ;
+
+
+    val_abs n e1 e2 : 
+      RE _ e1 e2 -> 
+      RV n (abs e1) (abs e2) ;
+
+    comp_ret n v1 v2 : 
+      RV _ v1 v2 ->
+      RE n (ret v1) (ret v2) ;
+
+    comp_let n e1 e2 e1' e2' : 
+      RE _ e1 e2 -> 
+      RE _ e1' e2' ->
+      RE n (let_ e1 e1') (let_ e2 e2') ;
+
+    comp_ifz n v1 v2 e1 e2 e1' e2' : 
+      RV _ v1 v2 -> 
+      RE _ e1 e2 -> 
+      RE _ e1' e2' -> 
+      RE n (ifz v1 e1 e1') (ifz v2 e2 e2') ;
+
+
+    comp_app n v1 v2 v1' v2' :
+      RV _ v1 v2 -> 
+      RV _ v1' v2' -> 
+      RE n (app v1 v1') (app v2 v2') ;
+
+
+}.
+
+(** * Contextual preorder definition *)
+
+Inductive CTX n (e e' : Tm n) : Prop := 
+  rel : forall RE RV, 
+      Compatible RE RV -> 
+      Adequate RE -> 
+      Transitive RE ->
+      RE n e e' -> CTX n e e'.
+
+(** * We want to know properties about CTX *)
+
+
+(** ---------------------------------------------------- * *)
+
+(* Any relation that is compatible is also reflexive *)
+
+Scheme Val_Tm_rec := Induction for Val Sort Prop 
+    with 
+    Tm_Val_rec := Induction for Tm Sort Prop.
+
+Combined Scheme Val_Tm_mutrec from 
+  Tm_Val_rec, Val_Tm_rec.
+
+Lemma Compatible_refl RE RV : 
+  Compatible RE RV -> 
+  forall n, (forall e, RE n e e) /\ (forall v, RV n v v).
+Proof. 
+  intros CC.
+  eapply Val_Tm_mutrec with 
+    (P0 := fun n t => RE n t t)
+    (P := fun n v => RV n v v).
+  all: intros.
+  - eapply val_var.
+  - eapply val_unit.
+  - eapply val_abs; eauto.
+  - eapply val_zero.
+  - eapply val_succ; eauto.
+(* FILL IN HERE *) Admitted.
+
+Instance Compatible_ReflexiveRE {RE}{RV} `{H : Compatible RE RV} : Reflexive RE.
+constructor. intro n.
+move: (Compatible_refl _ _ H) => h1.
+eapply (h1 n).
+Qed.
+
+Instance Compatible_ReflexiveRV {RE RV} `{H : Compatible RE RV} : Reflexive RV.
+constructor. intro n.
+move: (Compatible_refl _ _ H) => h1.
+eapply (h1 n).
+Qed.
+
+
+(* ------------------------------------------------------------------ *)
+
+(* We won't show that CTX is compatible here, but we can show that it 
+   is both Adequate and Transitive *)
+
+(** Adequacy of CTX is straightforward *)
+
+Instance Adequate_CTX : Adequate CTX.
+unfold Adequate.
+intros e e' h1 h.
+inversion h1.
+eapply H0; eauto.
+Qed.
+
+(* ------------------------------------------------------------------ *)
+
+(** Transtivity of CTX is more difficult to show *)
+
+Inductive OR_star {T : nat -> Type} (RE1 RE2: scoped_relation T) n (t1 t2 : T n) : Prop := 
+  | OR_1 : RE1 n t1 t2 -> OR_star RE1 RE2 n t1 t2 
+  | OR_2 : RE2 n t1 t2 -> OR_star RE1 RE2 n t1 t2 
+  | OR_trans t3 : 
+    OR_star RE1 RE2 n t1 t3
+    -> OR_star RE1 RE2 n t3 t2 
+    -> OR_star RE1 RE2 n t1 t2. 
+
+Instance Reflexive_OR_star {T} {RE1 RE2 : scoped_relation T} 
+  `{Reflexive T RE1} : Reflexive (OR_star RE1 RE2).
+Proof.
+constructor.
+- intros n t.
+  eapply OR_1; eapply scoped_refl; eauto.
+Qed.
+
+Instance Transitive_OR_star {T} {RE1 RE2 : scoped_relation T} :
+  Transitive (OR_star RE1 RE2).
+Proof.
+constructor.
+- intros n t1 t2 t3 O1 O2.    
+  eapply OR_trans; eauto.
+Qed.
+
+Instance PreOrder_OR_star {T} {RE1 RE2 : scoped_relation T} 
+  `{Reflexive T RE1} : 
+  PreOrder (OR_star RE1 RE2).
+split. constructor; eapply scoped_refl. constructor; eapply scoped_trans.
+Qed.
+
+Instance Adequate_OR_star {RE1 RE2 : scoped_relation Tm} `{Adequate RE1} `{Adequate RE2} : Adequate (OR_star RE1 RE2). 
+Proof.
+unfold Adequate in *.
+intros e e' O. induction O; eauto.
+Qed.
+
+Ltac compat_case H1 f := 
+induction H1; [ 
+  eapply OR_1; eapply f; eauto |
+  eapply OR_2; eapply f; eauto |
+  eapply OR_trans; eauto].
+
+
+Instance Compatible_OR_star 
+  {RE1 RE2 : scoped_relation Tm}
+  {RV1 RV2 : scoped_relation Val} 
+   `{PreOrder Tm RE1} `{PreOrder Tm RE2}
+   `{Reflexive _ RV1} `{Reflexive _ RV2}
+   `{Compatible RE1 RV1} `{Compatible RE2 RV2} : 
+  Compatible (OR_star RE1 RE2) (OR_star RV1 RV2).      
+Proof.               
+constructor.
+all: intros.
+- eapply OR_1; eapply val_var; eauto.
+- eapply OR_1; eapply val_unit; eauto.
+- eapply OR_1; eapply val_zero; eauto.
+- compat_case H5 @val_succ.
+(* FILL IN HERE *) Admitted.
+
+Instance Transitive_CTX : Transitive CTX.
+constructor.
+- intros n t1 t2 t3 C1 C2.
+  destruct C1 as [RE1 RV1 ? ? ? R1].
+  destruct C2 as [RE2 RV2 ? ? ? R2].
+  eapply (rel n t1 t3 (OR_star RE1 RE2) (OR_star RV1 RV2)).
+  + eapply Compatible_OR_star; eauto.
+    Unshelve. split; eauto. 
+    constructor. eapply scoped_refl. 
+    split; eauto.
+    constructor. eapply scoped_refl.
+  + eapply Adequate_OR_star; eauto.
+  + eapply PreOrder_OR_star; eauto.
+  + eapply OR_trans. eapply OR_1; eauto.
+    eapply OR_2; eauto.
+Qed.
+
+(** --------------------------------------------------------- *)
+
