rocq/untyped/equiv.v
@@ -1,0 +1,748 @@
+(** This development is adapted from Andy Pitts, 
+    "Step-Indexed Biorthogonality: a Tutorial Example" 
+
+    It demonstrates the use of a step-indexed logical 
+    relation to define contextual equivalence for the 
+    untyped lambda calculus.
+
+    The key ideas are 
+
+     (1) Definition of "Contextual" preorder as the largest 
+           adequate, compatible preorder
+     (2) Definition of "CIU" preorder 
+           what terms look the same with all stacks (uses), 
+           and after all substitutions (closing instantiations)
+     (3) Use of a step-indexed "logical" preorder to show
+           the equivalence between the two definitions    
+
+*)
+
+From Stdlib Require Import Psatz.
+From Stdlib Require Import Arith.
+
+Require Export common.core.
+Require Export untyped.stack.
+Require Import rec.iprop.
+
+Require Export untyped.ctx.
+
+Import SyntaxNotations.
+Import Lists.List.ListNotations.
+Import stack.Notations.
+Import rec.iprop.Notations.
+
+Open Scope list_scope.
+Open Scope rec_scope.
+
+(* -------------------------------------------------------- *)
+
+(** * Closed instantiations (of uses) *)
+
+Definition ciu : Tm 0 -> Tm 0 -> Prop := 
+  fun e e' => 
+    forall s, Small.halts (s, e) -> Small.halts (s, e').
+
+Definition CIU : scoped_relation Tm := 
+  fun n e e' => 
+    forall σ, ciu e[σ] e'[σ].
+
+(* By definition CIU is an adequate pre-order *)
+
+Instance Adequate_CIU : Adequate CIU.
+Proof.
+  intros e e' h.
+  unfold CIU, ciu in h.
+  unfold Small.halts.
+  specialize (h ids nil).
+  asimpl in h.
+  done.
+Qed.
+
+Instance Reflexive_CIU : Reflexive CIU.
+  constructor.
+  - intros n t. unfold CIU, ciu.
+    done.
+Qed.
+
+Instance Transitive_CIU : Transitive CIU.
+Proof.
+  constructor.
+  - intros n t1 t2 t3.
+    unfold CIU, ciu.
+    intros h1 h2 s E.
+    specialize (h1 s E).
+    specialize (h2 s E).
+    intro h; eauto.
+Qed.
+
+
+(** To show that CIU is compatible, we need to show that 
+    it is equivalent to an obviously compatible
+    logical relation. *)
+
+
+(*** ------------------ **)
+
+(** * Step-indexed logical relation *)
+
+
+(* Step-indexed relation *)
+Fixpoint V (v v' : Val 0) k {struct k} : Prop := 
+  let fix St (s s' : stack) k := 
+    ▷ (St s s') k /\
+    forall v v', (V v v') k ->
+            (fun k => Small.halts_n (s, ret v) k -> Small.halts (s', ret v')) k
+  in
+  let fix C (e e' : Tm 0) k := 
+    ▷ (C e e') k /\
+    forall s s' , (St s s') k ->
+             (fun k => Small.halts_n (s, e) k -> Small.halts (s', e')) k
+  in
+   match v , v' with 
+   | unit, unit => True
+   | zero, zero => True
+   | succ v1 , succ v2 => 
+       ▷ (V v1 v2) k
+   | abs e , v2 => 
+       ▷ (V v v') k /\
+       forall v1 v1', (▷ (V v1 v1') k ->
+                  ▷ (C e[v1 .: (abs e)..] (app v2 v1')) k)
+
+   | _ , _ => False
+   end.
+
+Fixpoint St (s s' : stack) k := 
+    ▷ (St s s') k /\
+    forall v v', (V v v') k ->
+            (fun k => Small.halts_n (s, ret v) k -> 
+                   Small.halts   (s', ret v')) k.
+Fixpoint C (e e' : Tm 0) k := 
+    ▷ (C e e') k /\
+    forall s s' , (St s s') k ->
+             (fun k => Small.halts_n (s, e) k -> Small.halts (s', e')) k.
+
+(* extended to open relations by closing over 
+   related substitutions *)
+
+Definition eqsig n (σ σ' : fin n -> Val 0) k :=
+    forall x, V (σ x) (σ' x) k.
+
+Definition eqval n (v v' : Val n) := 
+  forall k σ σ' , eqsig n σ σ' k -> V v[σ] v'[σ'] k.
+
+Definition eqtm  n (e e' : Tm n) := 
+  forall k σ σ' , eqsig n σ σ' k -> C e[σ] e'[σ'] k.
+  
+Definition eqst (s s' : stack) := 
+  forall k, St s s' k.
+
+(** * All step-indexed definitions are downward closed. *)
+
+Instance DownC e e' : IProp (C e e').
+constructor.  
+induction k.
+intros hC j LEj. inversion LEj. done.
+intros hC j LEj. inversion LEj. done.
+subst. cbn in hC. move: hC => [hC _].
+eapply IHk; eauto. 
+Qed.
+
+Instance DownSt E E' : IProp (St E E').
+constructor.
+induction k.
+intros hC j LEj. inversion LEj. done.
+intros hC j LEj. inversion LEj. done.
+subst. cbn in hC. move: hC => [hC _].
+eapply IHk; eauto. 
+Qed.
+
+Instance DownV v v' : IProp (V v v').
+constructor. move=> k. 
+move: v v'. 
+induction k; intros v v'.
+intros hC j LEj. inversion LEj. done.
+intros hC j LEj. inversion LEj. done.
+subst. 
+destruct v; destruct v'; try done.
+all: cbn in hC.
+all: try solve [next j; eapply IHk; eauto; lia].
+all: try solve [destruct hC; eapply IHk; eauto].
+all: try solve [destruct hC;
+  next j; split; [eauto | eapply IHk; auto]; lia].
+- next j. done.
+- next j. done.
+
+Qed.
+
+Instance Down_eqsig n σ σ' : IProp (eqsig n σ σ').
+constructor. 
+unfold eqsig.
+intros k EQ j LE x.
+eapply dclosed; eauto.
+Qed.
+
+(** * Convenience functions for unfolding the logical relation *)
+
+Lemma St_def : forall s s' k, 
+  St s s' k <-> 
+  (forall v v' , ((V v v') ⇒ 
+              (fun k => Small.halts_n (s, ret v) k -> Small.halts (s', ret v'))) k).
+Proof.
+  move=> E E'.
+  elim /strong_ind. intros k ih.
+  split.
+  - intros StEE.
+    intros v v' j LEj Vvv'.
+    inversion LEj. subst.
+    + destruct k; cbn in StEE;
+      move: StEE => [_ h];
+      specialize (h v v'); eapply h; eauto.
+    + subst.
+      specialize (ih j ltac:(lia)).
+      move: ih => [h1 h2].
+      eapply h1; eauto.
+      eapply dclosed; eauto.
+  - intros h.
+    destruct k.
+    + split; auto. done.
+      intros v v' Vv'. eapply h; eauto.
+    + split; auto. cbn.
+      specialize (ih k ltac:(auto)). rewrite ih.
+      intros v v' j LEj. eapply h; eauto.
+      intros v v' Vvv'. eapply h; eauto.
+Qed.
+    
+Lemma C_def (e e' : Tm 0) k :
+ C e e' k <->  
+   (forall s s' , ((St s s') ⇒ 
+              (fun k => Small.halts_n (s, e) k -> Small.halts (s', e'))) k).
+Proof. 
+  move: k.
+  elim /strong_ind. intros k ih.
+  split.
+  - intros Cee'.
+    intros E E' j LEj StEE'.
+    inversion LEj; subst.
+    + destruct k; eapply Cee'; auto.
+    + specialize (ih j ltac:(lia)).
+      eapply ih; eauto.
+      eapply dclosed; eauto.
+  - intros h.
+    destruct k; split; auto. 
+    done.
+    intros E E' StEE'.
+    eapply h; eauto.
+    specialize (ih k ltac:(auto)). cbn. rewrite ih.
+    intros E E' j LEj. eapply h; eauto.
+    intros E E' StEE'. eapply h; eauto.
+Qed.
+
+Lemma V_def_abs e v2 k :
+   V (abs e) v2 k <-> 
+        forall v v', (▷ (V v v') ⇒ ▷ (C e[v .: (abs e)..] (app v2 v'))) k.
+move: k.
+elim /strong_ind. intros k ih.
+split.
+- intro Vabs.
+  intros v v' j LEj Vvv'.
+  next j. cbn in Vvv'.
+  inversion LEj. subst.
+  + cbn in Vabs. fold St C in Vabs. move: Vabs => [Vabs h].
+    eapply h; eauto.
+  + subst. specialize (ih (S j) ltac:(lia)).
+    move: ih => [h _].
+    apply dclosed with (j:= S j) in Vabs. 2: lia.
+    specialize (h Vabs v v' (S j) ltac:(auto) Vvv'). 
+    cbn. done.
+- intros h. 
+  next k. fold St C.
+  specialize (ih k ltac:(eauto)). 
+  split.
+  + rewrite ih.
+    intros v v' j LEj Vvv'. eapply h; eauto.
+  + intros v v' Vvv'.
+    specialize (h v v' (S k) ltac:(lia)). cbn in h. auto.
+Qed.
+
+
+Lemma V_def (v v' : Val 0) k :
+  V v v' k <->
+   match v , v' with 
+   | unit , unit => True 
+   | zero  , zero => True
+   | succ v1 , succ v2 => ▷ (V v1 v2) k
+   | abs e , _ => 
+       forall v1 v1', (▷ (V v1 v1') ⇒ ▷ (C e[v1 .: (abs e)..] (app v' v1'))) k
+
+   | _ , _ => False
+   end.
+Proof.
+  destruct v eqn:EV. 
+  all: try solve [destruct k; cbn; done].
+  rewrite V_def_abs. done.
+Qed.
+
+
+
+(** * Computation relation is closed under reverse eval *)
+
+Lemma reverse_prim2 e1 e2 e2' k : 
+  C e1 e2' k -> e2 ~>> e2' -> C e1 e2 k.
+Proof.
+  repeat rewrite C_def.
+  intros h hSS.
+  intros E E' j LEj StEE hEe1.
+  specialize (h _ _ j LEj StEE hEe1).
+  eapply Small.halts_reverse_prim; eauto.
+Qed.
+
+
+(** Two congruence lemmas for working with f_let frames and let_ terms *)
+
+Lemma E_LET_cong k e e' (s s' : stack) : 
+  (forall v v', (▷ (V v v') ⇒ ▷ (C e[v..] e'[v'..])) k) ->
+  ((St s s' ⇒ St (f_let e :: s) (f_let e' :: s')) k).
+Proof.
+  intro h17. 
+  intros j LEj Sts.
+  rewrite St_def.
+  intros v v' i LEi VVi hH.
+  edestruct @halts_n_forward with (m' := (s, e[v..])) as [k0 [EQ hH']]; 
+    eauto using Small.step. subst.
+
+  move: (h17 v v' (S k0) (ltac:(lia))) => h1. cbn in h1.
+  apply dclosed with (j := k0) in VVi; auto. 
+  specialize (h1 VVi). rewrite C_def in h1.
+  specialize (h1 s s' k0 ltac:(auto) ltac:(eapply dclosed; eauto; lia)).
+  cbn in h1.
+  eapply halts_reverse; eauto using stack.Small.step.
+Qed.
+
+
+Lemma E_let_cong k e e' e1 e1' : 
+  (forall v v', (▷ (V v v') ⇒ ▷ (C e[v..] e'[v'..])) k) ->
+  ((C e1 e1' ⇒ C (let_ e1 e) (let_ e1' e')) k).
+Proof. 
+  intro h17. 
+  intros j LEj hE.
+  rewrite C_def.
+  rewrite C_def in hE.
+  intros s s' i LEi EEi hH.
+  move: (E_LET_cong k e e' s s' h17) => hSt.
+
+  eapply @halts_n_forward with (m' := (f_let e :: s, e1)) in hH;
+    eauto using Small.step.  
+  edestruct hH as [k0 [<- h2]].
+
+  specialize (hSt k0 ltac:(lia) ltac:(eapply dclosed; eauto; lia)). 
+  rewrite St_def in hSt.
+
+  move: (hE (f_let e :: s) (f_let e' :: s') k0 ltac:(lia)) => he1.
+  have StLET: St (f_let e :: s) (f_let e' :: s') k0.
+  { rewrite St_def. intros v v' m LEm VVm hLET.
+    inversion hLET.
+    eapply hSt; eauto.
+  } 
+  specialize (he1 StLET h2).
+
+  eapply Small.halts_reverse; eauto using Small.step.
+Qed.
+
+(** * Compatibility rules: values *)
+
+Lemma eqvar n x : eqval n (var x) (var x).
+Proof.
+intros k σ σ' Es.
+cbn. unfold eqsig in Es. eauto.
+Qed.
+
+Lemma eqzero n : eqval n zero zero.
+Proof.
+intros k σ σ' Es.
+cbn. unfold eqsig in Es. eauto.
+next k. done.
+Qed.
+
+Lemma equnit n : eqval n unit unit.
+Proof.
+intros k σ σ' Es.
+cbn. unfold eqsig in Es. eauto.
+next k. done.
+Qed.
+
+Lemma eqsucc n v v' : 
+  eqval n v v' -> 
+  eqval n (succ v) (succ v').
+Proof.
+intro h.
+intros k σ σ' Es.
+cbn. unfold eqsig in Es.
+next k. eapply h. unfold eqsig.
+intros x. eapply dclosed. eauto. lia.
+Qed.
+
+Lemma subst_rewrite : forall {n} (σ : fin n -> Val 0) (e : Tm (S (S n)))  (v1 v2 : Val 0), 
+    e [⇑ (⇑ σ)][v1 .: v2..] = e [v1 .: (v2 .: σ)].
+intros.
+asimpl.
+done.
+Qed.
+
+
+Lemma eqabs n e e' : 
+  eqtm _ e e' ->
+  eqval n (abs e) (abs e').
+Proof.
+intro h.
+unfold eqval.
+(** we need to use strong induction because of recursive functions *)
+elim /strong_ind. intros k ih.
+intros σ σ' Es.
+cbn. rewrite V_def_abs.
+intros v v' j LEj Vv.
+rewrite subst_rewrite.
+next j.
+cbn in Vv.
+eapply reverse_prim2. 2: { econstructor. } 
+rewrite subst_rewrite.
+eapply h.
+unfold eqsig.
+intro x. destruct x; cbn; auto.
+destruct f; cbn; auto.
+eapply dclosed with (j:=j) in Es; eauto.
+lia. 
+specialize (ih j ltac:(lia) σ σ' ltac:(eapply dclosed; eauto; try lia)).
+cbn in ih.
+done.
+Qed.
+
+
+
+(** * Compatibility rules: terms *)
+
+Lemma eqret n v v' : 
+  eqval n v v' 
+  -> eqtm n (ret v) (ret v').  
+Proof.
+(* FILL IN HERE *) Admitted.
+
+
+(* Application is congruence *)
+Lemma eqapp n v1 v1' v2 v2' : 
+  eqval n v1 v1' -> eqval n v2 v2' ->
+  eqtm n (app v1 v2) (app v1' v2').
+Proof.
+(* FILL IN HERE *) Admitted.
+
+Lemma eqlet n e1 e1' e2 e2' : 
+  eqtm n e1 e1' -> eqtm (S n) e2 e2' -> 
+  eqtm n (let_ e1 e2) (let_ e1' e2').
+Proof.
+(* FILL IN HERE *) Admitted.
+
+
+Lemma eqifz n v v' e0 e0' e1 e1' : 
+  eqval n v v' -> eqtm n e0 e0' -> eqtm _ e1 e1' -> 
+  eqtm _ (ifz v e0 e1) (ifz v' e0' e1').
+Proof. 
+(* FILL IN HERE *) Admitted.
+
+
+
+Instance compat_eq : Compatible eqtm eqval.
+constructor.
+- eapply eqvar.
+- eapply equnit.
+- eapply eqzero.
+- eapply eqsucc.
+
+- eapply eqabs.
+
+- eapply eqret. 
+- eapply eqlet.
+- eapply eqifz.
+
+- eapply eqapp.
+
+Qed.
+
+(* --------------------------------------------- *)
+
+(** Because the logical relation is compatible, it is also 
+    reflexive. This is our fundamental property of the 
+    logical relation. *)
+
+Corollary refl_val n v : eqval n v v.
+Proof.
+  eapply scoped_refl; eauto.
+Qed.
+Corollary refl_tm n e : eqtm n e e.
+Proof.
+  eapply scoped_refl; eauto.
+Qed.
+
+Lemma refl_sig n s : forall k, eqsig n s s k.
+Proof.
+  intros k. unfold eqsig. 
+  intros x.
+  move: (refl_val 0 (s x)) => h.
+  unfold eqval in h.
+  specialize (h k ids ids). asimpl in h.
+  eapply h.
+  unfold eqsig. auto_case.
+Qed.
+
+Lemma refl_St E : eqst E E.
+Proof.
+(* FILL IN HERE *) Admitted.
+
+(* --------------------------------------------- *)
+
+(* Now that we have shown that the logical relation is 
+   reflexive, we can show that it is equivalent to CIU *)
+
+(** * Logical  preorder implies CIU pre-order *)
+Lemma eqtm_CIU n e e' : 
+  eqtm n e e' -> CIU n e e'.
+Proof.
+(* FILL IN HERE *) Admitted.
+
+(** * Logical preorder is closed under CIU *)
+Lemma eqtm_closed_CIU n e e' e'' :
+  eqtm n e e' -> CIU n e' e'' -> eqtm n e e''.
+Proof. 
+(* FILL IN HERE *) Admitted.
+
+
+(** * CIU Pre-order implies logical preorder *)
+Lemma CIU_eqtm n e e' : 
+  CIU n e e' -> eqtm n e e'.
+Proof.
+  intros h.
+  move: (refl_tm n e) => hE.
+  eapply eqtm_closed_CIU; eauto.
+Qed.
+
+
+(* -------------------------------------------- *)
+
+(** Because CIU is equivalent to to logical equivalence, we can 
+now show that it is compatible. *)
+
+Instance Compatible_CIU : Compatible CIU eqval.
+constructor.
+- eapply eqvar; eauto.
+- eapply equnit; eauto.
+- eapply eqzero; eauto.
+- eapply eqsucc; eauto.
+
+- intros n e1 e2 CIU.
+  eapply eqabs.
+  eapply CIU_eqtm; auto.
+
+- intros.
+  eapply eqtm_CIU.
+  eapply eqret; eauto.
+- intros.
+  eapply eqtm_CIU.
+  eapply eqlet; eauto using CIU_eqtm.
+- intros. 
+  eapply eqtm_CIU.
+  eapply eqifz; eauto using CIU_eqtm.
+
+- intros.
+  eapply eqtm_CIU.
+  eapply eqapp; eauto.
+
+Qed.
+
+(** Compatibilility was the last piece of showing that 
+    CIU implies CTX. *)
+
+Lemma CIU_CTX n e e' : 
+  CIU n e e' -> CTX n e e'.
+Proof.
+  intros h.
+  econstructor; eauto.
+  - eapply Compatible_CIU.
+  - eapply Adequate_CIU.
+  - eapply Transitive_CIU.
+Qed.
+
+
+(* -------------------------------------------- *)
+
+(* TO Show that CTX implies CIU, we need to know that 
+   CTX is closed under substitution. *)
+
+
+(* We show this by induction on the length of the substitution. 
+   For a single step, we use the transtivity of CTX to 
+   make the chain:
+
+       e[v..] == (let (ret v) e) == (let (ret v) e') == e'[v..]
+ *)
+
+Lemma substitutivity n e e' v : 
+  CTX (S n) e e' ->
+  CTX n e[v..] e'[v..].
+Proof.
+  intro h.
+  have C1: CTX n (let_ (ret v) e) (let_ (ret v) e').
+  { 
+    destruct h.
+    econstructor; eauto.
+    eapply comp_let.
+    eapply comp_ret.
+    eapply scoped_refl; eauto.
+    done.
+  } 
+  have C2 : CTX n e[v..] (let_ (ret v) e).
+  { 
+    eapply CIU_CTX.
+    unfold CIU. intros s.
+    unfold ciu.
+    intros E.
+    asimpl.
+    intro h1.
+    eapply halts_reverse; 
+      [| eauto using stack.Small.step, primitive].
+    eapply halts_reverse; 
+      [| eauto using stack.Small.step, primitive].
+    asimpl.
+    done.
+  } 
+  have C3 : CTX n (let_ (ret v) e') e'[v..].
+  { 
+    eapply CIU_CTX.
+    unfold CIU. intros s.
+    unfold ciu.
+    intros E.
+    asimpl.
+    intro h1.
+    eapply halts_forward in h1;  
+      [| eauto using stack.Small.step, primitive].
+    eapply halts_forward in h1;  
+      [| eauto using stack.Small.step, primitive].
+    asimpl in h1.
+    done.
+  } 
+  eapply scoped_trans; eauto.
+  eapply scoped_trans; eauto.
+Qed.
+
+
+Lemma split_sigma (n : nat) (e : Tm (S n)) (σ : fin (S n) -> Val 0) :
+  e[(σ var_zero)⟨null⟩..][↑ >> σ] = e[σ].
+Proof. 
+  asimpl.
+  rewrite idSubst_Val. auto_case.
+  asimpl.
+  auto.
+Qed.
+
+Lemma value_substitutivity n e e' : 
+  CTX n e e' -> 
+  forall σ, CTX 0 e[σ] e'[σ].
+Proof.
+  move: e e'.
+  induction n.
+  all: intros e e' h σ.
+  - auto_unfold. 
+    repeat rewrite idSubst_Tm; try auto_case. auto.
+  - remember ((σ var_zero)⟨null⟩ : Val n) as v.
+    specialize (IHn e[v..] e'[v..]).
+    have h1:  CTX n e[v..] e'[v..].
+    { eapply substitutivity; eauto. } 
+    specialize (IHn h1 (↑ >> σ)).
+    rewrite Heqv in IHn.
+    repeat rewrite split_sigma in IHn.
+    auto.    
+Qed.
+
+Lemma halts_LET s e' e : 
+  Small.halts (f_let e' :: s, e) <-> Small.halts (s,let_ e e').
+Proof.
+  split.
+  - intro h. eapply halts_reverse; 
+      eauto using stack.Small.step, primitive.
+  - intro h. eapply halts_forward; 
+      eauto using stack.Small.step, primitive.
+Qed.
+
+Lemma CTX_ciu e e' :
+  CTX 0 e e' -> ciu e e'.
+Proof. 
+  intros h.
+  inversion h. clear h.
+  unfold ciu.
+  intros s.
+  move: e e' H2.
+  induction s; intros e e' Re.
+  - specialize (H0 _ _ Re) => A.
+    eauto.
+  - destruct a.
+    repeat rewrite halts_LET.
+    intro h1.
+    move: (@comp_let _ _ H) => CC.
+    have Rtt: RE 1 t t. eapply scoped_refl.
+    specialize (CC 0 e e' t t Re Rtt).
+    move: (IHs _ _ CC) => h2.
+    auto.
+Qed.
+
+
+Lemma CTX_CIU n e e' :
+  CTX n e e' -> CIU n e e'.
+Proof. 
+  intros h.
+  unfold CIU.
+  intros σ.
+  eapply CTX_ciu.
+  eapply value_substitutivity.
+  eauto.
+Qed.
+
+
+(** -------------------------------------------------------- *)
+
+(** Now we have that all of our preorders are equivalent. *)
+
+Lemma eqtm_CTX n e e' : 
+  eqtm n e e' -> CTX n e e'.
+Proof. intro h. eapply CIU_CTX. eapply eqtm_CIU. auto. Qed.
+Lemma CTX_eqtm n e e' :
+  CTX n e e' -> eqtm n e e'.
+Proof. intro h. eapply CIU_eqtm. eapply CTX_CIU. auto. Qed.
+
+
+Instance Compatible_CTX : Compatible CTX eqval.
+constructor.
+- eapply eqvar; eauto.
+- eapply equnit; eauto.
+- eapply eqzero; eauto.
+- eapply eqsucc; eauto.
+
+- intros n e1 e2 CTX.
+  eapply eqabs.
+  eapply CTX_eqtm; auto.
+
+- intros.
+  eapply eqtm_CTX.
+  eapply eqret; eauto.
+- intros.
+  eapply eqtm_CTX.
+  eapply eqlet; eauto using CTX_eqtm.
+- intros. 
+  eapply eqtm_CTX.
+  eapply eqifz; eauto using CTX_eqtm.
+
+- intros.
+  eapply eqtm_CTX.
+  eapply eqapp; eauto.
+
+Qed.
+
+
+(** -------------------------------------------------------- *)
+
