rocq/untyped/stack.v
@@ -1,0 +1,132 @@
+Require Export untyped.prim.
+
+Import SyntaxNotations.
+Import Lists.List.ListNotations.
+Open Scope list_scope.
+Open Scope rec_scope.
+
+(** * Semantics based on an abstract machine with an explicit stack *)
+
+(** A frame corresponds to the [let_cong] rule of the small step semantics.
+   It remembers that after evaluating [e1] we need to continue with evaluting
+   the body of a let expression. This body has a single bound variable. *)
+
+Definition frame   := Frame 0.
+Definition stack   := list frame.
+Definition machine := (stack * Tm 0)%type.
+
+(** An abstract machine is done evaluating when the stack is empty and 
+    the expression is a value. *)
+Inductive final : machine -> Prop := 
+  | final_machine v :
+    final ( [] , ret v ).
+
+Module Small.
+
+Local Reserved Notation "m ↦ m'" (at level 70).
+
+Inductive step : machine -> machine -> Prop := 
+  | s_prim s e e' : 
+    e ~>> e' ->
+    (s , e) ↦ (s, e')
+
+  | s_pop s e2 v : 
+    (f_let e2 :: s, ret v) ↦ (s, e2[v..])
+
+  | s_push  s e1 e2 : 
+    (s , let_ e1 e2 ) ↦ (f_let e2 :: s, e1)
+where "m ↦ m'" := (step m m') : rec_scope.
+  
+Definition irreducible (m : machine) : Prop := 
+  forall m', not (m ↦ m').
+
+Lemma deterministic :
+  forall m m1 m2, (m ↦ m1) -> (m ↦ m2) -> m1 = m2.
+Proof.
+  intros m m1 m2 h1 h2. 
+  inversion h1; subst; inversion h2; subst; auto.
+  all: try match goal with [ H : ret _ ~>> _ |- _ ] => inversion H end.
+  all: try match goal with [ H : let_ _ _ ~>> _ |- _ ] => inversion H end.
+  eapply primitive_deterministic in H; eauto. subst. auto.
+Qed.
+
+
+Definition halts_n (m : machine) n : Prop := 
+  exists v, step_n step n m (nil, ret v).
+
+Definition halts (m : machine) : Prop := 
+  exists v, multi step m (nil, ret v).
+
+Lemma halts_reverse_prim s e e' : 
+  halts (s, e') ->
+  e ~>> e' ->
+  halts (s, e).
+Proof.
+  intros h ss.
+  destruct h as [m sn].
+  exists m. econstructor; eauto. econstructor; eauto.
+Qed.
+
+Lemma halts_reverse m m' : 
+  halts m ->
+  m' ↦ m ->
+  halts m'.
+Proof.
+  intros h ss.
+  destruct h as [k sn].
+  exists k. econstructor; eauto. 
+Qed.
+
+End Small.
+
+Module Notations.
+Infix "↦"  := Small.step (at level 70) : rec_scope.
+Infix "↦*" := (multi Small.step) (at level 70) : rec_scope.
+End Notations.
+
+Import Notations.
+
+Lemma terminal_halts {v} : 
+  Small.halts (nil, ret v).
+Proof.
+  exists v. eapply ms_refl; eauto.
+Qed.
+
+Lemma halts_reverse {m m'}:
+  Small.halts m' ->  m ↦ m' ->
+  Small.halts m.
+Proof.
+  intros [v h] ss.
+  exists v. econstructor; eauto.
+Qed.
+
+
+Lemma halts_forward {m m'}:
+  Small.halts m -> m ↦ m' -> 
+  Small.halts m'.
+Proof.
+  intros h ss.
+  inversion h; subst. inversion H; subst. inversion ss. inversion H3.
+  apply Small.deterministic with (m1 := e2) in ss; eauto. subst.
+  eexists. eauto.
+Qed.
+
+Lemma halts_n_forward {m m' k}:
+  Small.halts_n m k -> m ↦ m' -> 
+  exists j, S j = k /\ Small.halts_n m'  j.
+Proof.
+  intros h ss.
+  inversion h; subst. inversion H; subst. inversion ss. inversion H3.
+  apply Small.deterministic with (m1 := e2) in ss; eauto. subst.
+  eexists. split; eauto. econstructor; eauto. 
+Qed.
+
+Lemma halts_n_reverse {m m' k}:
+  Small.halts_n m'  k ->  m ↦ m' ->
+  Small.halts_n m (S k).
+Proof.
+  intros [v h] ss.
+  exists v. econstructor; eauto.
+Qed.
+
+
